feat(init/meta/interactive): multiple subst
This allows `subst a, subst b, subst c` to be written `subst a b c`. This fixes a flaw in the previous version of this PR as part of #1777, by parsing expressions at max prec rather than identifiers, so that notation like `subst h1 h2 ‹_ = _›` works as expected.

library/init/meta/interactive.lean
@@ -919,8 +919,8 @@ tactic.ac_refl
 meta def cc : tactic unit :=
 tactic.cc
 
-meta def subst (q : parse texpr) : tactic unit :=
-i_to_expr q >>= tactic.subst >> try (tactic.reflexivity reducible)
+meta def subst (l : parse parser.pexpr*) : tactic unit :=
+l.mmap' $ λ q, i_to_expr q >>= tactic.subst >> try (tactic.reflexivity reducible)
 
 meta def clear : parse ident* → tactic unit :=
 tactic.clear_lst
