tests/lean/run/simulate_on.lean
@@ -5,3 +5,11 @@ begin
   guard_target b + 0 + 0 = b,
   reflexivity
 end
+
+example (a b c : nat) : a = 0 → b = 1 → c = 0 → b + a + c = b :=
+begin
+  intros h1 h2 h3,
+  subst h1 h3,
+  guard_target b + 0 + 0 = b,
+  reflexivity
+end
